Sorting/MergeSortSpec.v
@@ -1,0 +1,123 @@
+Add Rec LoadPath "/home/zeimer/Code/Coq".
+
+Require Import MergeSort.
+
+Set Implicit Arguments.
+
+(* TODO *) Theorem merge_sorted : forall (A : LinDec) (l1 l2 : list A),
+    sorted A l1 -> sorted A l2 -> sorted A (merge A l1 l2).
+Proof.
+  intros A l1 l2 H. generalize dependent l2.
+  induction H.
+    destruct l2; auto.
+    induction 1; simpl in *; dec.
+    induction 1.
+      simpl. auto.
+      specialize (IHsorted _ (sorted1 A x0)). simpl in *. dec.
+      simpl.
+Restart.
+  induction l1 as [| h1 t1].
+    destruct l2; simpl; auto.
+    destruct l2; simpl; auto.
+      dec; intros.
+        
+    
+Abort.
+
+Lemma merge_In :
+  forall (A : LinDec) (x : A) (l1 l2 : list A),
+    In x (merge A l1 l2) <-> In x (l1 ++ l2).
+Proof.
+Admitted.
+
+Theorem msFun_In :
+  forall (A : LinDec) (x : A) (l : list A),
+    In x (msFun A l) -> In x l.
+Proof.
+  intros A x. apply (well_founded_ind (@lengthOrder_wf A)
+    (fun l : list A => In x (msFun A l) -> In x l)).
+  destruct x0 as [| h t]; intro IH.
+    inversion 1.
+    intro. rewrite msFun_equation in H. destruct t.
+      assumption.
+      apply merge_In in H. apply in_app_or in H. destruct H.
+        apply IH in H.
+          eapply take_In. eassumption.
+          apply take_length_lt. apply lt_div2. simpl. omega.
+        apply IH in H.
+          eapply drop_In. eassumption.
+          apply drop_length_lt; simpl; intuition. inversion H0.
+Qed.
+
+Theorem msFun_In_conv :
+  forall (A : LinDec) (x : A) (l : list A),
+   In x l -> In x (msFun A l).
+Proof.
+  intros A x. apply (well_founded_ind (@lengthOrder_wf A)
+    (fun l : list A => In x l -> In x (msFun A l))).
+  destruct x0 as [| h t]; intro IH.
+    inversion 1.
+    intro. rewrite msFun_equation. destruct t.
+      assumption.
+      rewrite merge_In. apply in_or_app. destruct (LinDec_eqb_spec _ x h).
+        left. apply IH.
+          apply take_length_lt. apply lt_div2. simpl. omega.
+          simpl. auto.
+        inversion H; subst.
+          contradiction.
+          apply IH in H0.
+            Focus 2. red; simpl; omega.
+            apply msFun_In in H0.
+            apply IH in H0. rewrite msFun_equation in H0. destruct t.
+              simpl. right. auto.
+              rewrite merge_In in H0. apply in_app_or in H0. destruct H0.
+                left. apply IH.
+                  apply take_length_lt. apply lt_div2. simpl. omega.
+Restart.
+  intros A x. apply (well_founded_ind (@lengthOrder_wf A)
+    (fun l : list A => In x l -> In x (msFun A l))).
+  destruct x0 as [| h t]; intro IH.
+    inversion 1.
+    intro. rewrite msFun_equation. destruct t.
+      assumption.
+      rewrite merge_In. apply in_or_app. inversion H; subst.
+        left. apply IH.
+          apply take_length_lt. apply lt_div2. simpl; omega.
+          simpl. auto.
+        inversion H0; subst.
+          destruct t using list_ind2; auto.
+            right. rewrite msFun_equation. simpl. dec.
+            left. apply IH.
+              apply take_length_lt. apply lt_div2. simpl; omega.
+              simpl. auto.
+          apply IH in H1.
+            Focus 2. red; simpl; omega.
+            rewrite msFun_equation in H1. destruct t using list_ind2.
+              Focus 3.
+Restart.
+  intros A x. apply (well_founded_ind (@lengthOrder_wf A)
+    (fun l : list A => In x l -> In x (msFun A l))).
+  destruct x0 using list_ind2; intro IH; simpl; destruct 1; subst; auto.
+    rewrite msFun_equation. rewrite merge_In. apply in_or_app. left.
+      apply IH.
+        apply take_length_lt. apply lt_div2. simpl; omega.
+        simpl. auto.
+    destruct H; subst.
+      rewrite msFun_equation. rewrite merge_In. apply in_or_app.
+        destruct x1 using list_ind2.
+          right. simpl. auto.
+          right. simpl. rewrite msFun_equation. dec.
+          left. apply IH.
+            apply take_length_lt. apply lt_div2. simpl; omega.
+            simpl. auto.
+      rewrite msFun_equation. rewrite merge_In. apply in_or_app.
+        destruct x1 using list_ind2.
+          inversion H.
+          simpl in H. destruct H; inversion H; subst. right. simpl.
+            rewrite msFun_equation. dec.
+          clear IHx1. apply IH in H.
+            Focus 2. red; simpl; omega.
+            rewrite msFun_equation, merge_In in H. apply in_app_or in H.
+              destruct H.
+                simpl in H. apply msFun_In in H. inversion H; subst.
+Abort.
